examples/Online/DY.Online.Run.fst
@@ -8,12 +8,41 @@ open DY.Online.Protocol
 
 let run () : traceful (option unit ) =
   let _ = IO.debug_print_string "************* Trace *************\n" in
+
+
   let alice = "alice" in
   let bob = "bob" in
 
-  let* (alice_sid, ping_ts) = send_ping alice bob in
-  let*? (bob_sid, ack_ts) = receive_ping_and_send_ack___ bob ping_ts in
-  let*? _ = receive_ack alice ack_ts in
+  // Generate private key for Alice
+  let* alice_global_session_priv_key_id = initialize_private_keys alice in
+  generate_private_key alice alice_global_session_priv_key_id (LongTermPkEncKey key_tag);*
+  
+  // Generate private key for Bob
+  let* bob_global_session_priv_key_id = initialize_private_keys bob in
+  generate_private_key bob bob_global_session_priv_key_id (LongTermPkEncKey key_tag);*
+
+  // Store Bob's public key in Alice's state
+  // 1. Initialize Alice's session to store public keys
+  // 2. Retrieve Bob's private key from his session
+  // 3. Compute the public key from the private key
+  // 4. Install Bob's public key in Alice's public key store
+  let* alice_global_session_pub_key_id = initialize_pki alice in
+  let*? priv_key_bob = get_private_key bob bob_global_session_priv_key_id (LongTermPkEncKey key_tag) in
+  let pub_key_bob = pk priv_key_bob in
+  install_public_key alice alice_global_session_pub_key_id (LongTermPkEncKey key_tag) bob pub_key_bob;*
+
+  // Store Alice's public key in Bob's state
+  let* bob_global_session_pub_key_id = initialize_pki bob in
+  let*? priv_key_alice = get_private_key alice alice_global_session_priv_key_id (LongTermPkEncKey key_tag) in
+  let pub_key_alice = pk priv_key_alice in
+  install_public_key bob bob_global_session_pub_key_id (LongTermPkEncKey key_tag) alice pub_key_alice;*
+
+  let alice_global_session_ids: global_sess_ids = {pki=alice_global_session_pub_key_id; private_keys=alice_global_session_priv_key_id} in
+  let bob_global_session_ids: global_sess_ids = {pki=bob_global_session_pub_key_id; private_keys=bob_global_session_priv_key_id} in
+
+  let*? (alice_sid, ping_ts) = send_ping alice bob alice_global_session_pub_key_id in
+  let*? (bob_sid, ack_ts) = receive_ping_and_send_ack bob bob_global_session_ids ping_ts in
+  let*? _ = receive_ack alice alice_global_session_priv_key_id ack_ts in
 
   let* tr = get_trace in
   let _ = IO.debug_print_string (
